fips202/Keccak1600_arrays.ec
@@ -1,6 +1,7 @@
 from Jasmin require import JWord.
-from JazzEC require export Array5 Array24 Array25.
+from JazzEC require export Array5 Array24 Array25 Array200.
 
 op init_5_64 = Array5.init <:W64.t>.
 op init_24_64 = Array24.init <:W64.t>.
 op init_25_64 = Array25.init <:W64.t>.
+op init_200_8 = Array200.init <:W8.t>.
